Merge current Iris trunk.

theories/heap.v
@@ -47,7 +47,7 @@ Section definitions.
     proj2_sig heap_mapsto_aux.
 
   Definition heap_mapsto_vec (l : loc) (q : Qp) (vl : list val) : iProp Σ :=
-    ([★ list] i ↦ v ∈ vl, heap_mapsto (shift_loc l i) q v)%I.
+    ([∗ list] i ↦ v ∈ vl, heap_mapsto (shift_loc l i) q v)%I.
 
   Fixpoint inter (i0 : Z) (n : nat) : gmapR Z (exclR unitC) :=
     match n with O => ∅ | S n => <[i0 := Excl ()]>(inter (i0+1) n) end.
@@ -60,9 +60,9 @@ Section definitions.
     proj2_sig heap_freeable_aux.
 
   Definition heap_inv : iProp Σ :=
-    (∃ (σ:state) hF, ownP σ ★ own heap_name (● to_heap σ)
-                            ★ own heap_freeable_name (● hF)
-                            ★ ■ heap_freeable_rel σ hF)%I.
+    (∃ (σ:state) hF, ownP σ ∗ own heap_name (● to_heap σ)
+                            ∗ own heap_freeable_name (● hF)
+                            ∗ ■ heap_freeable_rel σ hF)%I.
   Definition heap_ctx : iProp Σ := inv heapN heap_inv.
 
   Global Instance heap_ctx_persistent : PersistentP heap_ctx.
@@ -78,14 +78,14 @@ Notation "l ↦{ q } v" := (heap_mapsto l q v)
   (at level 20, q at level 50, format "l  ↦{ q }  v") : uPred_scope.
 Notation "l ↦ v" := (heap_mapsto l 1 v) (at level 20) : uPred_scope.
 
-Notation "l ↦★{ q } vl" := (heap_mapsto_vec l q vl)
-  (at level 20, q at level 50, format "l  ↦★{ q }  vl") : uPred_scope.
-Notation "l ↦★ vl" := (heap_mapsto_vec l 1 vl) (at level 20) : uPred_scope.
+Notation "l ↦∗{ q } vl" := (heap_mapsto_vec l q vl)
+  (at level 20, q at level 50, format "l  ↦∗{ q }  vl") : uPred_scope.
+Notation "l ↦∗ vl" := (heap_mapsto_vec l 1 vl) (at level 20) : uPred_scope.
 
-Notation "l ↦★{ q }: P" := (∃ vl, l ↦★{ q } vl ★ P vl)%I
-  (at level 20, q at level 50, format "l  ↦★{ q }:  P") : uPred_scope.
-Notation "l ↦★: P " := (∃ vl, l ↦★ vl ★ P vl)%I
-  (at level 20, format "l  ↦★:  P") : uPred_scope.
+Notation "l ↦∗{ q }: P" := (∃ vl, l ↦∗{ q } vl ∗ P vl)%I
+  (at level 20, q at level 50, format "l  ↦∗{ q }:  P") : uPred_scope.
+Notation "l ↦∗: P " := (∃ vl, l ↦∗ vl ∗ P vl)%I
+  (at level 20, format "l  ↦∗:  P") : uPred_scope.
 
 Notation "†{ q } l … n" := (heap_freeable l q n)
   (at level 20, q at level 50, format "†{ q } l … n") : uPred_scope.
@@ -117,19 +117,19 @@ Section heap.
   Global Instance heap_mapsto_timeless l q v : TimelessP (l↦{q}v).
   Proof. rewrite heap_mapsto_eq /heap_mapsto_def. apply _. Qed.
 
-  Global Instance heap_mapsto_vec_timeless l q vl : TimelessP (l ↦★{q} vl).
+  Global Instance heap_mapsto_vec_timeless l q vl : TimelessP (l ↦∗{q} vl).
   Proof. apply _. Qed.
 
   Global Instance heap_freeable_timeless q l n : TimelessP (†{q}l…n).
   Proof. rewrite heap_freeable_eq /heap_freeable_def. apply _. Qed.
 
-  Lemma heap_mapsto_op_eq l q1 q2 v : l ↦{q1} v ★ l ↦{q2} v ⊣⊢ l ↦{q1+q2} v.
+  Lemma heap_mapsto_op_eq l q1 q2 v : l ↦{q1} v ∗ l ↦{q2} v ⊣⊢ l ↦{q1+q2} v.
   Proof.
     by rewrite heap_mapsto_eq -own_op -auth_frag_op op_singleton pair_op dec_agree_idemp.
   Qed.
 
   Lemma heap_mapsto_op l q1 q2 v1 v2 :
-    l ↦{q1} v1 ★ l ↦{q2} v2 ⊣⊢ v1 = v2 ∧ l ↦{q1+q2} v1.
+    l ↦{q1} v1 ∗ l ↦{q2} v2 ⊣⊢ v1 = v2 ∧ l ↦{q1+q2} v1.
   Proof.
     destruct (decide (v1 = v2)) as [->|].
     { by rewrite heap_mapsto_op_eq pure_equiv // left_id. }
@@ -139,34 +139,34 @@ Section heap.
     rewrite op_singleton pair_op dec_agree_ne // singleton_valid. by intros [].
   Qed.
 
-  Lemma heap_mapsto_vec_nil l q : l ↦★{q} [] ⊣⊢ True.
+  Lemma heap_mapsto_vec_nil l q : l ↦∗{q} [] ⊣⊢ True.
   Proof. by rewrite /heap_mapsto_vec big_sepL_nil. Qed.
 
   Lemma heap_mapsto_vec_app l q vl1 vl2 :
-    l ↦★{q} (vl1 ++ vl2) ⊣⊢ l ↦★{q} vl1 ★ shift_loc l (length vl1) ↦★{q} vl2.
+    l ↦∗{q} (vl1 ++ vl2) ⊣⊢ l ↦∗{q} vl1 ∗ shift_loc l (length vl1) ↦∗{q} vl2.
   Proof.
     rewrite /heap_mapsto_vec big_sepL_app.
     do 2 f_equiv. intros k v. by rewrite shift_loc_assoc_nat.
   Qed.
 
-  Lemma heap_mapsto_vec_singleton l q v : l ↦★{q} [v] ⊣⊢ l ↦{q} v.
+  Lemma heap_mapsto_vec_singleton l q v : l ↦∗{q} [v] ⊣⊢ l ↦{q} v.
   Proof. by rewrite /heap_mapsto_vec big_sepL_singleton /= shift_loc_0. Qed.
 
   Lemma heap_mapsto_vec_cons l q v vl:
-    l ↦★{q} (v :: vl) ⊣⊢ l ↦{q} v ★ shift_loc l 1 ↦★{q} vl.
+    l ↦∗{q} (v :: vl) ⊣⊢ l ↦{q} v ∗ shift_loc l 1 ↦∗{q} vl.
   Proof.
     by rewrite (heap_mapsto_vec_app l q [v] vl) heap_mapsto_vec_singleton.
   Qed.
 
   Lemma heap_mapsto_vec_op_eq l q1 q2 vl :
-    l ↦★{q1} vl ★ l ↦★{q2} vl ⊣⊢ l ↦★{q1+q2} vl.
+    l ↦∗{q1} vl ∗ l ↦∗{q2} vl ⊣⊢ l ↦∗{q1+q2} vl.
   Proof.
     rewrite /heap_mapsto_vec -big_sepL_sepL. by setoid_rewrite heap_mapsto_op_eq.
   Qed.
 
   Lemma heap_mapsto_vec_op l q1 q2 vl1 vl2 :
     length vl1 = length vl2 →
-    l ↦★{q1} vl1 ★ l ↦★{q2} vl2 ⊣⊢ vl1 = vl2 ∧ l ↦★{q1+q2} vl1.
+    l ↦∗{q1} vl1 ∗ l ↦∗{q2} vl2 ⊣⊢ vl1 = vl2 ∧ l ↦∗{q1+q2} vl1.
   Proof.
     iIntros (Hlen%Forall2_same_length); iSplit.
     - revert l. induction Hlen as [|v1 v2 vl1 vl2 _ _ IH]=> l.
@@ -179,7 +179,7 @@ Section heap.
 
   Lemma heap_mapsto_vec_prop_op l q1 q2 n (Φ : list val → iProp Σ) :
     (∀ vl, Φ vl ⊢ length vl = n) →
-    l ↦★{q1}: Φ ★ l ↦★{q2}: (λ vl, length vl = n) ⊣⊢ l ↦★{q1+q2}: Φ.
+    l ↦∗{q1}: Φ ∗ l ↦∗{q2}: (λ vl, length vl = n) ⊣⊢ l ↦∗{q1+q2}: Φ.
   Proof.
     intros Hlen. iSplit.
     - iIntros "[Hmt1 Hmt2]".
@@ -193,16 +193,16 @@ Section heap.
       iSplitL "Hmt1 Hown"; iExists _; by iFrame.
   Qed.
 
-  Lemma heap_mapsto_op_split l q v : l ↦{q} v ⊣⊢ l ↦{q/2} v ★ l ↦{q/2} v.
+  Lemma heap_mapsto_op_split l q v : l ↦{q} v ⊣⊢ l ↦{q/2} v ∗ l ↦{q/2} v.
   Proof. by rewrite heap_mapsto_op_eq Qp_div_2. Qed.
 
   Lemma heap_mapsto_vec_op_split l q vl :
-    l ↦★{q} vl ⊣⊢ l ↦★{q/2} vl ★ l ↦★{q/2} vl.
+    l ↦∗{q} vl ⊣⊢ l ↦∗{q/2} vl ∗ l ↦∗{q/2} vl.
   Proof. by rewrite heap_mapsto_vec_op_eq Qp_div_2. Qed.
 
   Lemma heap_mapsto_vec_combine l q vl :
     vl ≠ [] →
-    l ↦★{q} vl ⊣⊢ own heap_name (◯ [⋅ list] i ↦ v ∈ vl,
+    l ↦∗{q} vl ⊣⊢ own heap_name (◯ [⋅ list] i ↦ v ∈ vl,
       {[shift_loc l i := (q, Cinr 0%nat, DecAgree v)]}).
   Proof.
     rewrite /heap_mapsto_vec heap_mapsto_eq /heap_mapsto_def /heap_mapsto_st=>?.
@@ -233,7 +233,7 @@ Section heap.
   Proof. revert i. induction n as [|n IH]=>i. done. by apply insert_valid. Qed.
 
   Lemma heap_freeable_op_eq l q1 q2 n n' :
-    †{q1}l…n ★ †{q2}shift_loc l n…n' ⊣⊢ †{q1+q2}l…(n+n').
+    †{q1}l…n ∗ †{q2}shift_loc l n…n' ⊣⊢ †{q1+q2}l…(n+n').
   Proof.
     by rewrite heap_freeable_eq /heap_freeable_def -own_op -auth_frag_op
       op_singleton pair_op inter_op.
@@ -305,8 +305,8 @@ Section heap.
   Lemma heap_alloc_vs σ l vl:
     (∀ m : Z, σ !! shift_loc l m = None) →
     own heap_name (● to_heap σ)
-    ==★ own heap_name (● to_heap (init_mem l vl σ))
-       ★ own heap_name (◯ [⋅ list] i ↦ v ∈ vl,
+    ==∗ own heap_name (● to_heap (init_mem l vl σ))
+       ∗ own heap_name (◯ [⋅ list] i ↦ v ∈ vl,
            {[shift_loc l i := (1%Qp, Cinr 0%nat, DecAgree v)]}).
   Proof.
     intros FREE. rewrite -own_op. apply own_update, auth_update_alloc.
@@ -325,12 +325,12 @@ Section heap.
   Lemma wp_alloc E n :
     nclose heapN ⊆ E → 0 < n →
     {{{ heap_ctx }}} Alloc (Lit $ LitInt n) @ E
-    {{{ l vl; LitV $ LitLoc l, n = length vl ★ †l…(Z.to_nat n) ★ l ↦★ vl }}}.
+    {{{ l vl, RET LitV $ LitLoc l; n = length vl ∗ †l…(Z.to_nat n) ∗ l ↦∗ vl }}}.
   Proof.
-    iIntros (???) "[#Hinv HΦ]". rewrite /heap_ctx /heap_inv.
+    iIntros (???) "#Hinv HΦ". rewrite /heap_ctx /heap_inv.
     iInv heapN as (σ hF) ">(Hσ & Hvalσ & HhF & %)" "Hclose".
-    iApply wp_alloc_pst=> //. iNext.
-    iIntros "{$Hσ}". iIntros (l σ') "(% & #Hσσ' & Hσ')".
+    iApply (wp_alloc_pst with "[$Hσ]")=> //.
+    iNext. iIntros (l σ') "(% & #Hσσ' & Hσ')".
     iDestruct "Hσσ'" as %(vl & HvlLen & Hvl).
     assert (vl ≠ []) by (intros ->; simpl in *; lia).
     iMod (heap_alloc_vs with "[$Hvalσ]") as "[Hvalσ' Hmapsto]"; first done.
@@ -347,9 +347,9 @@ Section heap.
   Qed.
 
   Lemma heap_free_vs l vl σ :
-    own heap_name (● to_heap σ) ★ own heap_name (◯ [⋅ list] i ↦ v ∈ vl,
+    own heap_name (● to_heap σ) ∗ own heap_name (◯ [⋅ list] i ↦ v ∈ vl,
       {[shift_loc l i := (1%Qp, Cinr 0%nat, DecAgree v)]})
-    ==★ own heap_name (● to_heap (free_mem l (length vl) σ)).
+    ==∗ own heap_name (● to_heap (free_mem l (length vl) σ)).
   Proof.
     rewrite -own_op. apply own_update, auth_update_dealloc.
     revert σ l. induction vl as [|v vl IH]=> σ l; [done|].
@@ -370,11 +370,11 @@ Section heap.
   Lemma wp_free E (n:Z) l vl :
     nclose heapN ⊆ E →
     n = length vl →
-    {{{ heap_ctx ★ ▷ l ↦★ vl ★ ▷ †l…(length vl) }}}
+    {{{ heap_ctx ∗ ▷ l ↦∗ vl ∗ ▷ †l…(length vl) }}}
       Free (Lit $ LitInt n) (Lit $ LitLoc l) @ E
-    {{{ ; LitV LitUnit, True }}}.
+    {{{ RET LitV LitUnit; True }}}.
   Proof.
-    iIntros (???Φ) "[(#Hinv & >Hmt & >Hf) HΦ]". rewrite /heap_ctx /heap_inv.
+    iIntros (???Φ) "(#Hinv & >Hmt & >Hf) HΦ". rewrite /heap_ctx /heap_inv.
     iInv heapN as (σ hF) ">(Hσ & Hvalσ & HhF & REL)" "Hclose". iDestruct "REL" as %REL.
     rewrite heap_freeable_eq /heap_freeable_def.
     iDestruct (own_valid_2 with "[$HhF $Hf]") as % [Hl Hv]%auth_valid_discrete_2.
@@ -384,9 +384,9 @@ Section heap.
     assert (vl ≠ []).
     { intros ->. by destruct (REL (l.1) (1%Qp, ∅)) as [[] ?]. }
     assert (0 < n) by (subst n; by destruct vl).
-    iApply (wp_free_pst _ σ); auto.
+    iApply (wp_free_pst _ σ with "[$Hσ]"). by auto.
     { intros i. subst n. eauto using heap_freeable_is_Some. }
-    iNext. iIntros "{$Hσ} Hσ". iMod (heap_free_vs with "[Hmt Hvalσ]") as "Hvalσ".
+    iNext. iIntros "Hσ". iMod (heap_free_vs with "[Hmt Hvalσ]") as "Hvalσ".
     { rewrite heap_mapsto_vec_combine //. iFrame. }
     iMod (own_update_2 with "[$HhF $Hf]") as "HhF".
     { apply auth_update_dealloc, (delete_singleton_local_update _ _ _). }
@@ -396,7 +396,7 @@ Section heap.
   Qed.
 
   Lemma heap_mapsto_lookup l ls q v σ:
-    own heap_name (● to_heap σ) ★
+    own heap_name (● to_heap σ) ∗
     own heap_name (◯ {[ l := (q, to_lock_stateR ls, DecAgree v) ]})
     ⊢ ■ ∃ n' : nat,
         σ !! l = Some (match ls with RSt n => RSt (n+n') | WSt => WSt end, v).
@@ -413,7 +413,7 @@ Section heap.
   Qed.
 
   Lemma heap_mapsto_lookup_1 l ls v σ:
-    own heap_name (● to_heap σ) ★
+    own heap_name (● to_heap σ) ∗
     own heap_name (◯ {[ l := (1%Qp, to_lock_stateR ls, DecAgree v) ]})
     ⊢ ■ (σ !! l = Some (ls, v)).
   Proof.
@@ -428,23 +428,23 @@ Section heap.
 
   Lemma wp_read_sc E l q v :
     nclose heapN ⊆ E →
-    {{{ heap_ctx ★ ▷ l ↦{q} v }}} Read ScOrd (Lit $ LitLoc l) @ E
-    {{{; v, l ↦{q} v }}}.
+    {{{ heap_ctx ∗ ▷ l ↦{q} v }}} Read ScOrd (Lit $ LitLoc l) @ E
+    {{{ RET v; l ↦{q} v }}}.
   Proof.
-    iIntros (??) "[[#Hinv >Hv] HΦ]".
+    iIntros (??) "[#Hinv >Hv] HΦ".
     rewrite /heap_ctx /heap_inv heap_mapsto_eq /heap_mapsto_def.
     iInv heapN as (σ hF) ">(Hσ & Hvalσ & HhF & %)" "Hclose".
     iDestruct (heap_mapsto_lookup with "[$Hvalσ $Hv]") as %[n Hσl].
-    iApply wp_read_sc_pst; first done. iNext. iIntros "{$Hσ} Hσ".
+    iApply (wp_read_sc_pst with "[$Hσ]"); first done. iNext. iIntros "Hσ".
     iMod ("Hclose" with "[-Hv HΦ]"); last by iApply "HΦ".
     iNext. iExists σ, hF. iFrame. eauto.
   Qed.
 
   Lemma heap_read_vs σ n1 n2 nf l q v:
     σ !! l = Some (RSt (n1 + nf), v) →
-    own heap_name (● to_heap σ) ★ heap_mapsto_st (RSt n1) l q v
-    ==★ own heap_name (● to_heap (<[l:=(RSt (n2 + nf), v)]> σ))
-        ★ heap_mapsto_st (RSt n2) l q v.
+    own heap_name (● to_heap σ) ∗ heap_mapsto_st (RSt n1) l q v
+    ==∗ own heap_name (● to_heap (<[l:=(RSt (n2 + nf), v)]> σ))
+        ∗ heap_mapsto_st (RSt n2) l q v.
   Proof.
     intros Hσv. rewrite -!own_op to_heap_insert.
     eapply own_update, auth_update, singleton_local_update.
@@ -455,10 +455,10 @@ Section heap.
 
   Lemma wp_read_na E l q v :
     nclose heapN ⊆ E →
-    {{{ heap_ctx ★ ▷ l ↦{q} v }}} Read Na1Ord (Lit $ LitLoc l) @ E
-    {{{; v, l ↦{q} v }}}.
+    {{{ heap_ctx ∗ ▷ l ↦{q} v }}} Read Na1Ord (Lit $ LitLoc l) @ E
+    {{{ RET v; l ↦{q} v }}}.
   Proof.
-    iIntros (??Φ) "[[#Hinv >Hv] HΦ]".
+    iIntros (??Φ) "[#Hinv >Hv] HΦ".
     rewrite /heap_ctx /heap_inv heap_mapsto_eq /heap_mapsto_def.
     iApply (wp_read_na1_pst E).
     iInv heapN as (σ hF) ">(Hσ & Hvalσ & HhF & %)" "Hclose".
@@ -471,7 +471,7 @@ Section heap.
     iModIntro. clear dependent n σ hF.
     iInv heapN as (σ hF) ">(Hσ & Hvalσ & HhF & %)" "Hclose".
     iDestruct (heap_mapsto_lookup with "[$Hvalσ $Hv]") as %[n Hσl].
-    iApply wp_read_na2_pst; first done. iNext. iIntros "{$Hσ} Hσ".
+    iApply (wp_read_na2_pst with "[$Hσ]"); first done. iNext. iIntros "Hσ".
     iMod (heap_read_vs with "[$Hvalσ $Hv]") as "[Hvalσ Hv]"; first done.
     iMod ("Hclose" with "[-Hv HΦ]") as "_"; last by iApply "HΦ".
     iNext. iExists _, hF. iFrame. eauto using heap_freeable_rel_stable.
@@ -479,9 +479,9 @@ Section heap.
 
   Lemma heap_write_vs σ st1 st2 l v v':
     σ !! l = Some (st1, v) →
-    own heap_name (● to_heap σ) ★ heap_mapsto_st st1 l 1%Qp v
-    ==★ own heap_name (● to_heap (<[l:=(st2, v')]> σ))
-        ★ heap_mapsto_st st2 l 1%Qp v'.
+    own heap_name (● to_heap σ) ∗ heap_mapsto_st st1 l 1%Qp v
+    ==∗ own heap_name (● to_heap (<[l:=(st2, v')]> σ))
+        ∗ heap_mapsto_st st2 l 1%Qp v'.
   Proof.
     intros Hσv. rewrite -!own_op to_heap_insert.
     eapply own_update, auth_update, singleton_local_update.
@@ -491,14 +491,14 @@ Section heap.
 
   Lemma wp_write_sc E l e v v' :
     nclose heapN ⊆ E → to_val e = Some v →
-    {{{ heap_ctx ★ ▷ l ↦ v' }}} Write ScOrd (Lit $ LitLoc l) e @ E
-    {{{; LitV LitUnit, l ↦ v }}}.
+    {{{ heap_ctx ∗ ▷ l ↦ v' }}} Write ScOrd (Lit $ LitLoc l) e @ E
+    {{{ RET LitV LitUnit; l ↦ v }}}.
   Proof.
-    iIntros (? <-%of_to_val?) "[[#Hinv >Hv] HΦ]".
+    iIntros (? <-%of_to_val?) "[#Hinv >Hv] HΦ".
     rewrite /heap_ctx /heap_inv heap_mapsto_eq /heap_mapsto_def.
     iInv heapN as (σ hF) ">(Hσ & Hvalσ & HhF & %)" "Hclose".
     iDestruct (heap_mapsto_lookup_1 with "[$Hvalσ $Hv]") as %?.
-    iApply wp_write_sc_pst; [done|]. iNext. iIntros "{$Hσ} Hσ".
+    iApply (wp_write_sc_pst with "[$Hσ]"); [done|]. iNext. iIntros "Hσ".
     iMod (heap_write_vs with "[$Hvalσ $Hv]") as "[Hvalσ Hv]"; first done.
     iMod ("Hclose" with "[-Hv HΦ]") as "_"; last by iApply "HΦ".
     iNext. iExists _, hF. iFrame. eauto using heap_freeable_rel_stable.
@@ -506,10 +506,10 @@ Section heap.
 
   Lemma wp_write_na E l e v v' :
     nclose heapN ⊆ E → to_val e = Some v →
-    {{{ heap_ctx ★ ▷ l ↦ v' }}} Write Na1Ord (Lit $ LitLoc l) e @ E
-    {{{; LitV LitUnit, l ↦ v }}}.
+    {{{ heap_ctx ∗ ▷ l ↦ v' }}} Write Na1Ord (Lit $ LitLoc l) e @ E
+    {{{ RET LitV LitUnit; l ↦ v }}}.
   Proof.
-    iIntros (? <-%of_to_val?) "[[#Hinv >Hv] HΦ]".
+    iIntros (? <-%of_to_val?) "[#Hinv >Hv] HΦ".
     rewrite /heap_ctx /heap_inv heap_mapsto_eq /heap_mapsto_def.
     iApply (wp_write_na1_pst E).
     iInv heapN as (σ hF) ">(Hσ & Hvalσ & HhF & %)" "Hclose".
@@ -522,7 +522,7 @@ Section heap.
     iModIntro. clear dependent σ hF.
     iInv heapN as (σ hF) ">(Hσ & Hvalσ & HhF & %)" "Hclose".
     iDestruct (heap_mapsto_lookup_1 with "[$Hvalσ $Hv]") as %?.
-    iApply wp_write_na2_pst; [done|]. iNext. iIntros "{$Hσ} Hσ".
+    iApply (wp_write_na2_pst with "[$Hσ]"); [done|]. iNext. iIntros "Hσ".
     iMod (heap_write_vs with "[$Hvalσ $Hv]") as "[Hvalσ Hv]"; first done.
     iMod ("Hclose" with "[-Hv HΦ]"); last by iApply "HΦ".
     iNext. iExists _, hF. iFrame. eauto using heap_freeable_rel_stable.
@@ -530,54 +530,53 @@ Section heap.
 
   Lemma wp_cas_int_fail E l q z1 e2 v2 zl :
     nclose heapN ⊆ E → to_val e2 = Some v2 → z1 ≠ zl →
-    {{{ heap_ctx ★ ▷ l ↦{q} (LitV $ LitInt zl) }}}
+    {{{ heap_ctx ∗ ▷ l ↦{q} (LitV $ LitInt zl) }}}
       CAS (Lit $ LitLoc l) (Lit $ LitInt z1) e2 @ E
-    {{{;LitV $ LitInt 0, l ↦{q} (LitV $ LitInt zl) }}}.
+    {{{ RET LitV $ LitInt 0; l ↦{q} (LitV $ LitInt zl) }}}.
   Proof.
-    iIntros (? <-%of_to_val ??) "[[#Hinv >Hv] HΦ]".
+    iIntros (? <-%of_to_val ??) "[#Hinv >Hv] HΦ".
     rewrite /heap_ctx /heap_inv heap_mapsto_eq /heap_mapsto_def.
     iInv heapN as (σ hF) ">(Hσ & Hvalσ & HhF & %)" "Hclose".
     iDestruct (heap_mapsto_lookup with "[$Hvalσ $Hv]") as %[n Hσl].
-    iApply wp_cas_fail_pst; eauto.
+    iApply (wp_cas_fail_pst with "[$Hσ]"); eauto.
     { by rewrite /= bool_decide_false. }
-    iNext. iIntros "{$Hσ} Hσ".
-    iMod ("Hclose" with "[-Hv HΦ]") as "_"; last by iApply "HΦ".
+    iNext. iIntros "Hσ". iMod ("Hclose" with "[-Hv HΦ]") as "_"; last by iApply "HΦ".
     iNext. iExists _, hF. iFrame. eauto using heap_freeable_rel_stable.
   Qed.
 
   Lemma wp_cas_loc_fail E l q q' q1 l1 v1' e2 v2 l' vl' :
     nclose heapN ⊆ E → to_val e2 = Some v2 → l1 ≠ l' →
-    {{{ heap_ctx ★ ▷ l ↦{q} (LitV $ LitLoc l') ★ ▷ l' ↦{q'} vl' ★ ▷ l1 ↦{q1} v1' }}}
+    {{{ heap_ctx ∗ ▷ l ↦{q} (LitV $ LitLoc l') ∗ ▷ l' ↦{q'} vl' ∗ ▷ l1 ↦{q1} v1' }}}
       CAS (Lit $ LitLoc l) (Lit $ LitLoc l1) e2 @ E
-    {{{;LitV $ LitInt 0,
-        l ↦{q} (LitV $ LitLoc l') ★ l' ↦{q'} vl' ★ l1 ↦{q1} v1' }}}.
+    {{{ RET LitV $ LitInt 0;
+        l ↦{q} (LitV $ LitLoc l') ∗ l' ↦{q'} vl' ∗ l1 ↦{q1} v1' }}}.
   Proof.
-    iIntros (? <-%of_to_val ??) "[(#Hinv & >Hl & >Hl' & >Hl1) HΦ]".
+    iIntros (? <-%of_to_val ??) "(#Hinv & >Hl & >Hl' & >Hl1) HΦ".
     rewrite /heap_ctx /heap_inv heap_mapsto_eq /heap_mapsto_def.
     iInv heapN as (σ hF) ">(Hσ & Hvalσ & HhF & %)" "Hclose".
     iDestruct (heap_mapsto_lookup with "[$Hvalσ $Hl]") as %[n Hσl].
     iDestruct (heap_mapsto_lookup with "[$Hvalσ $Hl']") as %[n' Hσl'].
     iDestruct (heap_mapsto_lookup with "[$Hvalσ $Hl1]") as %[n1 Hσl1].
-    iApply wp_cas_fail_pst; eauto.
+    iApply (wp_cas_fail_pst with "[$Hσ]"); eauto.
     { by rewrite /= bool_decide_false // Hσl1 Hσl'. }
-    iNext. iIntros "{$Hσ} Hσ ".
+    iNext. iIntros "Hσ ".
     iMod ("Hclose" with "[-Hl Hl' Hl1 HΦ]") as "_"; last by iApply "HΦ"; iFrame.
     iNext. iExists _, hF. by iFrame.
   Qed.
 
   Lemma wp_cas_int_suc E l z1 e2 v2 :
     nclose heapN ⊆ E → to_val e2 = Some v2 →
-    {{{ heap_ctx ★ ▷ l ↦ (LitV $ LitInt z1) }}}
+    {{{ heap_ctx ∗ ▷ l ↦ (LitV $ LitInt z1) }}}
       CAS (Lit $ LitLoc l) (Lit $ LitInt z1) e2 @ E
-    {{{; LitV $ LitInt 1, l ↦ v2 }}}.
+    {{{ RET LitV $ LitInt 1; l ↦ v2 }}}.
   Proof.
-    iIntros (? <-%of_to_val?) "[[#Hinv >Hv] HΦ]".
+    iIntros (? <-%of_to_val?) "[#Hinv >Hv] HΦ".
     rewrite /heap_ctx /heap_inv heap_mapsto_eq /heap_mapsto_def.
     iInv heapN as (σ hF) ">(Hσ & Hvalσ & HhF & %)" "Hclose".
     iDestruct (heap_mapsto_lookup_1 with "[$Hvalσ $Hv]") as %?.
-    iApply wp_cas_suc_pst; eauto.
+    iApply (wp_cas_suc_pst with "[$Hσ]"); eauto.
     { by rewrite /= bool_decide_true. }
-    iNext. iIntros "{$Hσ} Hσ".
+    iNext. iIntros "Hσ".
     iMod (heap_write_vs with "[$Hvalσ $Hv]") as "[Hvalσ Hv]"; first done.
     iMod ("Hclose" with "[-Hv HΦ]"); last by iApply "HΦ"; iFrame.
     iNext. iExists _, hF. iFrame. eauto using  heap_freeable_rel_stable.
@@ -585,17 +584,17 @@ Section heap.
 
   Lemma wp_cas_loc_suc E l l1 e2 v2 :
     nclose heapN ⊆ E → to_val e2 = Some v2 →
-    {{{ heap_ctx ★ ▷ l ↦ (LitV $ LitLoc l1) }}}
+    {{{ heap_ctx ∗ ▷ l ↦ (LitV $ LitLoc l1) }}}
       CAS (Lit $ LitLoc l) (Lit $ LitLoc l1) e2 @ E
-    {{{; LitV $ LitInt 1, l ↦ v2 }}}.
+    {{{ RET LitV $ LitInt 1; l ↦ v2 }}}.
   Proof.
-    iIntros (? <-%of_to_val?) "[[#Hinv >Hv] HΦ]".
+    iIntros (? <-%of_to_val?) "[#Hinv >Hv] HΦ".
     rewrite /heap_ctx /heap_inv heap_mapsto_eq /heap_mapsto_def.
     iInv heapN as (σ hF) ">(Hσ & Hvalσ & HhF & %)" "Hclose".
     iDestruct (heap_mapsto_lookup_1 with "[$Hvalσ $Hv]") as %?.
-    iApply wp_cas_suc_pst; eauto.
+    iApply (wp_cas_suc_pst with "[$Hσ]"); eauto.
     { by rewrite /= bool_decide_true. }
-    iNext. iIntros "{$Hσ} Hσ".
+    iNext. iIntros "Hσ".
     iMod (heap_write_vs with "[$Hvalσ $Hv]") as "[Hvalσ Hv]"; first done.
     iMod ("Hclose" with "[-Hv HΦ]"); last by iApply "HΦ"; iFrame.
     iNext. iExists _, hF. iFrame. eauto using  heap_freeable_rel_stable.
