theories/lifting.v
@@ -25,12 +25,12 @@ Proof. exact: weakestpre.wp_bind. Qed.
 Lemma wp_alloc_pst E σ n:
   0 < n →
   {{{ ▷ ownP σ }}} Alloc (Lit $ LitInt n) @ E
-  {{{ l σ'; LitV $ LitLoc l,
-      ■ (∀ m, σ !! (shift_loc l m) = None) ★
-      ■ (∃ vl, n = length vl ∧ init_mem l vl σ = σ') ★
+  {{{ l σ', RET LitV $ LitLoc l;
+      ■ (∀ m, σ !! (shift_loc l m) = None) ∗
+      ■ (∃ vl, n = length vl ∧ init_mem l vl σ = σ') ∗
       ownP σ' }}}.
 Proof.
-  iIntros (? Φ) "[HP HΦ]". iApply (wp_lift_atomic_head_step _ σ); eauto.
+  iIntros (? Φ) "HP HΦ". iApply (wp_lift_atomic_head_step _ σ); eauto.
   iFrame "HP". iNext. iIntros (v2 σ2 ef) "[% HP]". inv_head_step.
   rewrite big_sepL_nil right_id. by iApply "HΦ"; iFrame; eauto.
 Qed.
@@ -39,36 +39,36 @@ Lemma wp_free_pst E σ l n :
   0 < n →
   (∀ m, is_Some (σ !! (shift_loc l m)) ↔ (0 ≤ m < n)) →
   {{{ ▷ ownP σ }}} Free (Lit $ LitInt n) (Lit $ LitLoc l) @ E
-  {{{ ; LitV $ LitUnit, ownP (free_mem l (Z.to_nat n) σ) }}}.
+  {{{ RET LitV $ LitUnit; ownP (free_mem l (Z.to_nat n) σ) }}}.
 Proof.
-  iIntros (???)  "[HP HΦ]". iApply (wp_lift_atomic_head_step _ σ); eauto.
+  iIntros (???)  "HP HΦ". iApply (wp_lift_atomic_head_step _ σ); eauto.
   iFrame "HP". iNext. iIntros (v2 σ2 ef) "[% HP]". inv_head_step.
   rewrite big_sepL_nil right_id. by iApply "HΦ".
 Qed.
 
 Lemma wp_read_sc_pst E σ l n v :
   σ !! l = Some (RSt n, v) →
-  {{{ ▷ ownP σ }}} Read ScOrd (Lit $ LitLoc l) @ E {{{ ; v, ownP σ }}}.
+  {{{ ▷ ownP σ }}} Read ScOrd (Lit $ LitLoc l) @ E {{{ RET v; ownP σ }}}.
 Proof.
-  iIntros (??) "[?HΦ]". iApply wp_lift_atomic_det_head_step; eauto.
+  iIntros (??) "?HΦ". iApply wp_lift_atomic_det_head_step; eauto.
   by intros; inv_head_step; eauto using to_of_val.
-  rewrite big_sepL_nil right_id; iFrame. iNext. iIntros "?!>". by iApply "HΦ".
+  rewrite big_sepL_nil right_id; iFrame.
 Qed.
 
 Lemma wp_read_na2_pst E σ l n v :
   σ !! l = Some(RSt $ S n, v) →
   {{{ ▷ ownP σ }}} Read Na2Ord (Lit $ LitLoc l) @ E
-  {{{ ; v, ownP (<[l:=(RSt n, v)]>σ) }}}.
+  {{{ RET v; ownP (<[l:=(RSt n, v)]>σ) }}}.
 Proof.
-  iIntros (??) "[?HΦ]". iApply wp_lift_atomic_det_head_step; eauto.
+  iIntros (??) "?HΦ". iApply wp_lift_atomic_det_head_step; eauto.
   by intros; inv_head_step; eauto using to_of_val.
-  rewrite big_sepL_nil right_id; iFrame. iNext. iIntros "?!>". by iApply "HΦ".
+  rewrite big_sepL_nil right_id; iFrame.
 Qed.
 
 Lemma wp_read_na1_pst E l Φ :
   (|={E,∅}=> ∃ σ n v, σ !! l = Some(RSt $ n, v) ∧
-     ▷ ownP σ ★
-     ▷ (ownP (<[l:=(RSt $ S n, v)]>σ) ={∅,E}=★
+     ▷ ownP σ ∗
+     ▷ (ownP (<[l:=(RSt $ S n, v)]>σ) ={∅,E}=∗
           WP Read Na2Ord (Lit $ LitLoc l) @ E {{ Φ }}))
   ⊢ WP Read Na1Ord (Lit $ LitLoc l) @ E {{ Φ }}.
 Proof.
@@ -81,27 +81,25 @@ Qed.
 Lemma wp_write_sc_pst E σ l v v' :
   σ !! l = Some (RSt 0, v') →
   {{{ ▷ ownP σ }}} Write ScOrd (Lit $ LitLoc l) (of_val v) @ E
-  {{{ ; LitV LitUnit, ownP (<[l:=(RSt 0, v)]>σ) }}}.
+  {{{ RET LitV LitUnit; ownP (<[l:=(RSt 0, v)]>σ) }}}.
 Proof.
-  iIntros (??) "[?HΦ]". iApply wp_lift_atomic_det_head_step; eauto.
+  iIntros (??) "?HΦ". iApply wp_lift_atomic_det_head_step; eauto.
   by intros; inv_head_step; eauto. rewrite big_sepL_nil right_id; iFrame.
-  iNext. iIntros "?!>". by iApply "HΦ".
 Qed.
 
 Lemma wp_write_na2_pst E σ l v v' :
   σ !! l = Some(WSt, v') →
   {{{ ▷ ownP σ }}} Write Na2Ord (Lit $ LitLoc l) (of_val v) @ E
-  {{{ ; LitV LitUnit, ownP (<[l:=(RSt 0, v)]>σ) }}}.
+  {{{ RET LitV LitUnit; ownP (<[l:=(RSt 0, v)]>σ) }}}.
 Proof.
-  iIntros (??) "[?HΦ]". iApply wp_lift_atomic_det_head_step; eauto.
-  by intros; inv_head_step; eauto.
-  rewrite big_sepL_nil right_id; iFrame. iNext. iIntros "?!>". by iApply "HΦ".
+  iIntros (??) "?HΦ". iApply wp_lift_atomic_det_head_step; eauto.
+  by intros; inv_head_step; eauto. rewrite big_sepL_nil right_id; iFrame.
 Qed.
 
 Lemma wp_write_na1_pst E l v Φ :
   (|={E,∅}=> ∃ σ v', σ !! l = Some(RSt 0, v') ∧
-     ▷ ownP σ ★
-     ▷ (ownP (<[l:=(WSt, v')]>σ) ={∅,E}=★
+     ▷ ownP σ ∗
+     ▷ (ownP (<[l:=(WSt, v')]>σ) ={∅,E}=∗
        WP Write Na2Ord (Lit $ LitLoc l) (of_val v) @ E {{ Φ }}))
   ⊢ WP Write Na1Ord (Lit $ LitLoc l) (of_val v) @ E {{ Φ }}.
 Proof.
@@ -116,11 +114,11 @@ Lemma wp_cas_fail_pst E σ l n e1 v1 v2 vl :
   σ !! l = Some (RSt n, vl) →
   value_eq σ v1 vl = Some false →
   {{{ ▷ ownP σ }}} CAS (Lit $ LitLoc l) e1 (of_val v2) @ E
-  {{{ ; LitV $ LitInt 0, ownP σ }}}.
+  {{{ RET LitV $ LitInt 0; ownP σ }}}.
 Proof.
-  iIntros (?%of_to_val ???) "[HP HΦ]". subst.
+  iIntros (?%of_to_val ???) "HP HΦ". subst.
   iApply wp_lift_atomic_det_head_step; eauto. by intros; inv_head_step; eauto.
-  iFrame. iNext. rewrite big_sepL_nil right_id. iIntros "?!>". by iApply "HΦ".
+  iFrame. iNext. rewrite big_sepL_nil right_id. iIntros "?". by iApply "HΦ".
 Qed.
 
 Lemma wp_cas_suc_pst E σ l e1 v1 v2 vl :
@@ -128,18 +126,18 @@ Lemma wp_cas_suc_pst E σ l e1 v1 v2 vl :
   σ !! l = Some (RSt 0, vl) →
   value_eq σ v1 vl = Some true →
   {{{ ▷ ownP σ }}} CAS (Lit $ LitLoc l) e1 (of_val v2) @ E
-  {{{ ; LitV $ LitInt 1, ownP (<[l:=(RSt 0, v2)]>σ) }}}.
+  {{{ RET LitV $ LitInt 1; ownP (<[l:=(RSt 0, v2)]>σ) }}}.
 Proof.
-  iIntros (?%of_to_val ???) "[HP HΦ]". subst.
+  iIntros (?%of_to_val ???) "HP HΦ". subst.
   iApply wp_lift_atomic_det_head_step; eauto. by intros; inv_head_step; eauto.
-  iFrame. iNext. rewrite big_sepL_nil right_id. iIntros "?!>". by iApply "HΦ".
+  iFrame. iNext. rewrite big_sepL_nil right_id. iIntros "?". by iApply "HΦ".
 Qed.
 
 (** Base axioms for core primitives of the language: Stateless reductions *)
 Lemma wp_fork E e :
-  {{{ ▷ WP e {{ _, True }} }}} Fork e @ E {{{ ; LitV LitUnit, True }}}.
+  {{{ ▷ WP e {{ _, True }} }}} Fork e @ E {{{ RET LitV LitUnit; True }}}.
 Proof.
-  iIntros (?) "[?HΦ]". iApply wp_lift_pure_det_head_step; eauto.
+  iIntros (?) "?HΦ". iApply wp_lift_pure_det_head_step; eauto.
   by intros; inv_head_step; eauto. iNext.
   rewrite big_sepL_singleton. iFrame. iApply wp_value. done. by iApply "HΦ".
 Qed.
