theories/memcpy.v
@@ -20,9 +20,9 @@ Notation "e1 <-[ i ]{ n } ! e2" :=
 Lemma wp_memcpy `{heapG Σ} E l1 l2 vl1 vl2 q n:
   nclose heapN ⊆ E →
   length vl1 = n → length vl2 = n →
-  {{{ heap_ctx ★ l1 ↦★ vl1 ★ l2 ↦★{q} vl2 }}}
+  {{{ heap_ctx ∗ l1 ↦∗ vl1 ∗ l2 ↦∗{q} vl2 }}}
     #l1 <-{n} !#l2 @ E
-  {{{; #(), l1 ↦★ vl2 ★ l2 ↦★{q} vl2 }}}.
+  {{{; #(), l1 ↦∗ vl2 ∗ l2 ↦∗{q} vl2 }}}.
 Proof.
   iIntros (? Hvl1 Hvl2 Φ) "[(#Hinv & Hl1 & Hl2) HΦ]".
   iLöb as "IH" forall (n l1 l2 vl1 vl2 Hvl1 Hvl2). wp_rec. wp_op=> ?; wp_if.
